TCP Packets done.

src/BinEncoders/Env/Lib2/Option.v
@@ -1,5 +1,6 @@
 Require Import
         Fiat.Common
+        Fiat.Computation
         Fiat.Computation.Notations
         Fiat.BinEncoders.Env.Common.Specs
         Fiat.BinEncoders.Env.Common.WordFacts.
@@ -14,14 +15,91 @@ Section Option.
   Context {cacheAddNat : CacheAdd cache nat}.
   Context {transformer : Transformer B}.
 
-  Variable encode_A : A -> CacheEncode -> Comp (B * CacheEncode).
-  
   Definition encode_option_Spec
-             (encode_None : CacheEncode -> Comp (B * CacheEncode))
+             (encode_Some : A -> CacheEncode -> Comp (B * CacheEncode))
+             (encode_None : () -> CacheEncode -> Comp (B * CacheEncode))
              (a_opt : option A)
-    := match a_opt with
-       | Some a => encode_A a
-       | None => encode_None
-       end.
+    := If_Opt_Then_Else a_opt encode_Some (encode_None ()).
+
+  Lemma option_encode_correct
+      {P  : CacheDecode -> Prop}
+      {P_invT P_invE : (CacheDecode -> Prop) -> Prop}
+      (P_inv_pf : cache_inv_Property P (fun P => P_invT P /\ P_invE P))
+      (predicate_Some : A -> Prop)
+      (predicate_None : () -> Prop)
+      (b' : bool)
+      (predicate :=
+         fun a_opt =>
+           decides (negb b') (a_opt = None)
+           /\ match a_opt with
+              | Some a => predicate_Some a
+              | None => predicate_None ()
+              end)
+      (predicate_rest_Some : A -> B -> Prop)
+      (predicate_rest_None : () -> B -> Prop)
+      (predicate_rest :=
+         fun a_opt =>
+           match a_opt with
+           | Some a => predicate_rest_Some a
+           | None => predicate_rest_None ()
+           end)
+      (encode_Some : A -> CacheEncode -> Comp (B * CacheEncode))
+      (decode_Some : B -> CacheDecode -> option (A * B * CacheDecode))
+      (encode_None : () -> CacheEncode -> Comp (B * CacheEncode))
+      (decode_None : B -> CacheDecode -> option (() * B * CacheDecode))
+      (decode_Some_pf :
+         cache_inv_Property P P_invT
+         -> encode_decode_correct_f
+              cache transformer predicate_Some predicate_rest_Some
+              encode_Some decode_Some P)
+      (decode_None_pf :
+         cache_inv_Property P P_invE
+         -> encode_decode_correct_f
+              cache transformer predicate_None predicate_rest_None
+              encode_None decode_None P)
+  : encode_decode_correct_f
+      cache transformer
+      predicate
+      predicate_rest
+      (encode_option_Spec encode_Some encode_None)%comp
+      (fun (b : B) (env : CacheDecode) =>
+         If b' Then
+            match decode_Some b env with
+            | Some (a, b, c) => Some (Some a, b, c)
+            | None => None
+            end
+            Else
+            match decode_None b env with
+            | Some (a, b, c) => Some (None, b, c)
+            | None => None
+            end
+      ) P.
+Proof.
+  unfold cache_inv_Property in *; split.
+  { intros env env' xenv data bin ext env_pm pred_pm pred_pm_rest com_pf.
+    unfold encode_option_Spec in com_pf; computes_to_inv;
+      destruct data;
+      find_if_inside; unfold predicate in *; simpl in *;
+        intuition; try discriminate.
+    - eapply H3 in com_pf; destruct_ex;
+        intuition eauto; rewrite H6; eauto.
+    - eapply H4 in com_pf; destruct_ex;
+        intuition eauto; rewrite H6; eauto.
+  }
+  { intros.
+    find_if_inside; simpl in *.
+    - destruct (decode_Some bin env') as [ [ [? ?] ?] | ] eqn : ? ;
+        simpl in *; try discriminate; injections; simpl.
+      eapply decode_Some_pf in Heqo; intuition eauto.
+      destruct_ex; intuition; subst.
+      eexists _; eexists _; unfold predicate; intuition eauto.
+      discriminate.
+    - destruct (decode_None bin env') as [ [ [? ?] ?] | ] eqn : ? ;
+        simpl in *; try discriminate; injections; destruct u.
+      eapply decode_None_pf in Heqo; intuition eauto; destruct_ex;
+        intuition eauto; subst.
+      eexists _; eexists _; unfold predicate; intuition eauto.
+  }
+Qed.
 
 End Option.
